LeanMiniscript.lean
@@ -2,6 +2,7 @@ import LeanMiniscript.Script.Syntax
 import LeanMiniscript.Script.Assembly
 import LeanMiniscript.Script.ControlFlow
 import LeanMiniscript.Script.State
+import LeanMiniscript.Script.SignatureEncoding
 import LeanMiniscript.Script.Serialization
 import LeanMiniscript.Miniscript.KeyExpr
 import LeanMiniscript.Miniscript.Syntax
